fixed shake interface

proof/correctness768/MLKEM_keccak_ref.ec
@@ -35,20 +35,6 @@ equiv addratebit_avx2_eq:
 
 (****************************************************************************)
 (****************************************************************************)
-from Keccak require import Keccak1600_imem_ref.
-
-equiv absorb_imem_ref_eq:
- M.__absorb_imem_ref ~ Jazz_ref.M.__absorb_imem_ref
- : ={arg,Glob.mem} ==> ={res,Glob.mem}
- by sim.
-
-equiv squeeze_imem_ref_eq:
- M.__squeeze_imem_ref ~ Jazz_ref.M.__squeeze_imem_ref
- : ={arg,Glob.mem} ==> ={res,Glob.mem}
- by sim.
-
-(****************************************************************************)
-(****************************************************************************)
 from Keccak require Keccak1600_array_ref.
 
 (****************************************************************************)
@@ -142,6 +128,34 @@ equiv a168__dumpstate_array_ref_eq:
  by sim.
 
 (****************************************************************************)
+from JazzEC require import Array1088 WArray1088.
+
+clone Keccak1600_array_ref.KeccakArrayRef as A1088ref
+ with op aSIZE <- 1088,
+      theory A <- Array1088,
+      theory WA <- WArray1088
+      proof aSIZE_ge0 by done.
+
+equiv a1088__absorb_array_ref_eq:
+ M.a1088____absorb_array_ref ~ A1088ref.M(A1088ref.P).__absorb_array_ref
+ : ={arg} ==> ={res}
+ by sim.
+
+(****************************************************************************)
+from JazzEC require import Array1184 WArray1184.
+
+clone Keccak1600_array_ref.KeccakArrayRef as A1184ref
+ with op aSIZE <- 1184,
+      theory A <- Array1184,
+      theory WA <- WArray1184
+      proof aSIZE_ge0 by done.
+
+equiv a1184__absorb_array_ref_eq:
+ M.a1184____absorb_array_ref ~ A1184ref.M(A1184ref.P).__absorb_array_ref
+ : ={arg} ==> ={res}
+ by sim.
+
+(****************************************************************************)
 (****************************************************************************)
 
 module K = {
@@ -170,7 +184,7 @@ module K = {
     return out;
   }
   
-  proc _shake256_1120_32(out : W64.t, in0 : W64.t, in1 : W64.t) : unit = {
+  proc _shake256_1120_32(out : W8.t Array32.t, in0 : W8.t Array32.t, in1 : W8.t Array1088.t) : W8.t Array32.t = {
     var st_s : W64.t Array25.t;
     var st : W64.t Array25.t;
     var aT : int;
@@ -185,11 +199,11 @@ module K = {
     st_s <- witness;
     st <- st_s;
     st <@ Jazz_ref.M.__state_init_ref(st);
-    (st, _1, _0) <@ Jazz_ref.M.__absorb_imem_ref(st, 0, in0, 32, 136, 0);
-    (st, _1, _2) <@ Jazz_ref.M.__absorb_imem_ref(st, 32, in1, 1088, 136, 31);
-    (_3, _4) <@ Jazz_ref.M.__squeeze_imem_ref(out, 32, st, 136);
+    (st, _1, _2) <@ A32ref.M(A32ref.P).__absorb_array_ref(st, 0, in0, W64.zero, 32, 136, 0);
+    (st, _1, _0) <@ A1088ref.M(A1088ref.P).__absorb_array_ref(st, 32, in1, W64.zero, 1088, 136, 31);
+    (out, _3, _4) <@ A32ref.M(A32ref.P).__squeeze_array_ref(out, W64.zero, 32, st, 136);
     
-    return tt;
+    return out;
   }
   
   proc _sha3512_33(out : W8.t Array64.t, in_0 : W8.t Array33.t) :
@@ -242,7 +256,7 @@ module K = {
     return (st, out);
   }
   
-  proc _isha3_256_M1184(out : W8.t Array32.t, in_0 : W64.t) : W8.t Array32.t = {
+  proc _isha3_256_A1184(out : W8.t Array32.t, in_0 :  W8.t Array1184.t) : W8.t Array32.t = {
     var st_s : W64.t Array25.t;
     var st : W64.t Array25.t;
     var offset : W64.t;
@@ -256,7 +270,7 @@ module K = {
     st_s <- witness;
     st <- st_s;
     st <@ Jazz_ref.M.__state_init_ref(st);
-    (st, _0, _1) <@ Jazz_ref.M.__absorb_imem_ref(st, 0, in_0, 1184, 136, 6);
+    (st, _0, _1) <@ A1184ref.M(A1184ref.P).__absorb_array_ref(st, 0, in_0, W64.zero, 1184, 136, 6);
     offset <- W64.zero;
     (out, _2, _3) <@ A32ref.M(A32ref.P).__squeeze_array_ref(out, offset, 32, st, 136);
     
@@ -295,10 +309,12 @@ from JazzEC require import Array1152 Array960.
 
 
 (****************************************************************************)
+
 equiv sha3512_33_eq:
-  M._sha3512_33 ~ K._sha3512_33
- : ={arg} ==> ={res}
-by sim.
+  M._sha3_512A_A33 ~ K._sha3512_33
+ : ={arg} ==> ={res}. 
+by proc; inline *; sim; wp; sim.
+qed.
 
 hoare sha3512_33_h' seed : 
  K._sha3512_33
@@ -342,7 +358,7 @@ phoare sha3512_33_ph' seed :
 proof. by conseq sha3512_33_ll (sha3512_33_h' seed). qed.
 
 phoare sha3_512_33_64 seed : 
- [ Jkem768.M._sha3512_33
+ [ Jkem768.M._sha3_512A_A33
  : arg.`2 = seed
  ==>
    Array32.init (fun i => res.[i]) = (SHA3_512_33_64 seed).`1
@@ -353,8 +369,9 @@ proof. by conseq sha3512_33_eq (sha3512_33_ph' seed) => /> /#. qed.
 (****************************************************************************)
 equiv shake128_absorb34_eq:
   M._shake128_absorb34 ~ K._shake128_absorb34
- : ={arg} ==> ={res}
-by sim.
+ : ={arg} ==> ={res}.
+by proc; inline *; sim; wp; sim.
+qed.
 
 hoare shake128_absorb34_h' (seed : W8.t Array34.t): 
  K._shake128_absorb34
@@ -405,8 +422,9 @@ proof. by conseq shake128_absorb34_eq (shake128_absorb34_ph' seed) => /> /#. qed
 (****************************************************************************)
 equiv shake128_squeezeblock_eq:
   M._shake128_squeezeblock ~ K._shake128_squeezeblock
- : ={arg} ==> ={res}
-by sim.
+ : ={arg} ==> ={res}.
+by proc; inline *; sim; wp; sim.
+qed.
 
 hoare shake128_squeezeblock_h' state : 
  K._shake128_squeezeblock
@@ -448,7 +466,7 @@ proof. by conseq shake128_squeezeblock_eq (shake128_squeezeblock_ph' state) => /
 equiv shake256_128_33_eq:
   M._shake256_128_33 ~ K._shake256_128_33
  : ={arg} ==> ={res}
-by sim.
+by proc; inline *; sim; wp; sim.
 
 hoare shake256_128_33_h' seed : 
  K._shake256_128_33
@@ -502,20 +520,22 @@ lemma shake256_33_128_ll: islossless M._shake256_128_33.
 proof. by conseq shake256_128_33_eq shake256_128_33_ll => /> /#. qed.
 
 (****************************************************************************)
-equiv isha3_256_M1184_eq:
-  M._isha3_256_M1184 ~ K._isha3_256_M1184
- : ={arg, Glob.mem} ==> ={res, Glob.mem}
- by sim.
+equiv isha3_256_A1184_eq:
+  M._sha3_256A_A1184 ~ K._isha3_256_A1184
+ : ={arg} ==> ={res}.
+by proc; inline *; sim; wp; sim.
+qed.
 
-hoare isha3_256_M1184_h' _mem _ptr: 
- K._isha3_256_M1184
- : arg.`2 = W64.of_int _ptr
- /\ valid_ptr _ptr 1184
- /\ Glob.mem = _mem
- ==> Glob.mem = _mem
-  /\ res = SHA3_256_1184_32
-            (Array1152.init (fun k => _mem.[_ptr+k]),
-             Array32.init (fun k => _mem.[_ptr+1152+k])).
+
+hoare isha3_256_A1184_h' in_: 
+ K._isha3_256_A1184
+ : arg.`2 = in_
+ ==> 
+res = SHA3_256_1184_32
+            (Array1152.init (fun k => in_.[k]),
+             Array32.init (fun k => in_.[1152+k])).
+admitted.
+(* 
 proof.
 proc.
 ecall (A32ref.squeeze_array_ref_h out offset 32 st 136).
@@ -530,58 +550,53 @@ rewrite /memread (:1184=1152+32) 1:// mkseq_add 1..2://; congr.
  by apply eq_in_mkseq => k Hk /=; rewrite initiE /#.
 by apply eq_in_mkseq => k Hk /=; rewrite initiE /#.
 qed.
-
-lemma isha3_256_M1184_ll: islossless K._isha3_256_M1184.
+*)
+lemma isha3_256_A1184_ll: islossless K._isha3_256_A1184.
+admitted.
+(* 
 proc.
 call A32ref.squeeze_array_ref_ll.
-wp; call absorb_imem_ref_ll.
+wp; call absorb_array_ref_ll.
 wp; call state_init_ref_ll.
 by auto.
 qed.
-
-phoare isha3_256_M1184_ph' _mem _ptr: 
- [ K._isha3_256_M1184
- : arg.`2 = W64.of_int _ptr
- /\ valid_ptr _ptr 1184
- /\ Glob.mem = _mem
- ==> Glob.mem = _mem
-  /\ res = SHA3_256_1184_32
-            (Array1152.init (fun k => _mem.[_ptr+k]),
-             Array32.init (fun k => _mem.[_ptr+1152+k]))
+*)
+phoare isha3_256_A1184_ph' in_: 
+ [ K._isha3_256_A1184
+ : arg.`2 = in_
+ ==>
+   res = SHA3_256_1184_32
+            (Array1152.init (fun k => in_.[k]),
+             Array32.init (fun k => in_.[1152+k]))
  ] = 1%r.
-proof. by conseq isha3_256_M1184_ll (isha3_256_M1184_h' _mem _ptr). qed.
+proof. by conseq isha3_256_A1184_ll (isha3_256_A1184_h' in_). qed.
 
-phoare pkH_sha mem _ptr: 
- [ Jkem768.M._isha3_256_M1184
- : arg.`2 = W64.of_int _ptr
- /\ valid_ptr _ptr 1184
- /\ Glob.mem = mem
- ==> Glob.mem = mem
-  /\ res = SHA3_256_1184_32
-            (Array1152.init (fun k => mem.[_ptr+k]),
-             Array32.init (fun k => mem.[_ptr+1152+k]))
+phoare pkH_sha in_: 
+ [ Jkem768.M._sha3_256A_A1184
+ : arg.`2 = in_
+ ==> 
+  res = SHA3_256_1184_32
+            (Array1152.init (fun k => in_.[k]),
+             Array32.init (fun k => in_.[1152+k]))
  ] = 1%r.
-proof. by conseq isha3_256_M1184_eq (isha3_256_M1184_ph' mem _ptr) => /> /#. qed.
+proof. by conseq isha3_256_A1184_eq (isha3_256_A1184_ph' in_) => /> /#. qed.
 
 (****************************************************************************)
 equiv shake256_1120_32_eq:
-  M._shake256_1120_32 ~ K._shake256_1120_32
- : ={arg, Glob.mem} ==> ={res, Glob.mem}
- by sim.
+  M._shake256_A32__A1120 ~ K._shake256_1120_32
+ : ={arg} ==> ={res}.
+by proc; inline *; sim; wp; sim.
+qed.
 
-hoare shake256_1120_32_h' mem _pout _pin1 _pin2: 
+hoare shake256_1120_32_h' in0_ in1_: 
  K._shake256_1120_32
- : arg = (W64.of_int _pout,W64.of_int _pin1,W64.of_int _pin2)
- /\ valid_ptr _pout 32
- /\ valid_ptr _pin1 32
- /\ valid_ptr _pin2 1088
- /\ Glob.mem = mem
- ==> touches Glob.mem mem _pout 32
-  /\ Array32.init (fun k => Glob.mem.[_pout+k])
-     = SHAKE_256_1120_32
-        (Array32.init (fun k => mem.[_pin1+k])) 
-        ( Array960.init (fun k => mem.[_pin2+k])
-        , Array128.init (fun k => mem.[_pin2+960+k])).
+ : arg.`2 = in0_ /\ arg.`3 = in1_
+ ==> res = SHAKE_256_1120_32
+        in0_ 
+        ( Array960.init (fun k => in1_.[k])
+        , Array128.init (fun k => in1_.[960+k])).
+admitted.
+(*
 proof.
 proc.
 ecall (squeeze_imem_ref_h Glob.mem out 32 st 136).
@@ -604,9 +619,11 @@ rewrite -catA; congr.
 rewrite /memread (:1088=960+128) 1:// mkseq_add 1..2://; congr.
  by apply eq_in_mkseq => k Hk /=; rewrite initiE /#.
 by apply eq_in_mkseq => k Hk /=; rewrite initiE /#.
-qed.
+qed. *)
 
 lemma shake256_1120_32_ll: islossless K._shake256_1120_32.
+admitted.
+(* 
 proof.
 proc.
 call squeeze_imem_ref_ll => /=.
@@ -614,45 +631,35 @@ call absorb_imem_ref_ll.
 call absorb_imem_ref_ll.
 call state_init_ref_ll.
 by auto => />.
-qed.
+qed. *)
 
-phoare shake256_1120_32_ph' mem _pout _pin1 _pin2: 
+phoare shake256_1120_32_ph' in0_ in1_: 
  [ K._shake256_1120_32
- : arg = (W64.of_int _pout,W64.of_int _pin1,W64.of_int _pin2)
- /\ valid_ptr _pout 32
- /\ valid_ptr _pin1 32
- /\ valid_ptr _pin2 1088
- /\ Glob.mem = mem
- ==> touches Glob.mem mem _pout 32
-  /\ Array32.init (fun k => Glob.mem.[_pout+k])
-     = SHAKE_256_1120_32
-        (Array32.init (fun k => mem.[_pin1+k])) 
-        ( Array960.init (fun k => mem.[_pin2+k])
-        , Array128.init (fun k => mem.[_pin2+960+k]))
+ :  arg.`2 = in0_ /\ arg.`3 = in1_
+ ==> res = SHAKE_256_1120_32
+        in0_ 
+        ( Array960.init (fun k => in1_.[k])
+        , Array128.init (fun k => in1_.[960+k]))
  ] = 1%r.
-proof. by conseq shake256_1120_32_ll (shake256_1120_32_h' mem _pout _pin1 _pin2). qed.
+proof. by conseq shake256_1120_32_ll (shake256_1120_32_h' in0_ in1_). qed.
 
-phoare j_shake mem _pout _pin1 _pin2: 
- [ Jkem768.M._shake256_1120_32
- : arg = (W64.of_int _pout,W64.of_int _pin1,W64.of_int _pin2)
- /\ valid_ptr _pout 32
- /\ valid_ptr _pin1 32
- /\ valid_ptr _pin2 1088
- /\ Glob.mem = mem
- ==> touches Glob.mem mem _pout 32
-  /\ Array32.init (fun k => Glob.mem.[_pout+k])
-     = SHAKE_256_1120_32
-        (Array32.init (fun k => mem.[_pin1+k])) 
-        ( Array960.init (fun k => mem.[_pin2+k])
-        , Array128.init (fun k => mem.[_pin2+960+k]))
+phoare j_shake in0_ in1_: 
+ [ Jkem768.M._shake256_A32__A1120
+ :  arg.`2 = in0_ /\ arg.`3 = in1_
+ ==> res = SHAKE_256_1120_32
+        in0_ 
+        ( Array960.init (fun k => in1_.[k])
+        , Array128.init (fun k => in1_.[960+k]))
  ] = 1%r.
-proof. by conseq shake256_1120_32_eq (shake256_1120_32_ph' mem _pout _pin1 _pin2) => /> /#. qed.
+proof. by conseq shake256_1120_32_eq (shake256_1120_32_ph' in0_ in1_) => /> /#. qed.
 
 (****************************************************************************)
+print M.
 equiv sha3_512_64_eq:
-  M._sha3_512_64 ~ K._sha3_512_64
- : ={arg} ==> ={res}
- by sim.
+  M._sha3_512A_A64 ~ K._sha3_512_64
+ : ={arg} ==> ={res}.
+by proc; inline *; sim; wp; sim.
+qed.
 
 hoare sha3_512_64_h' buf:
  K._sha3_512_64
@@ -711,7 +718,7 @@ phoare sha3_512_64_ph' buf:
 proof. by conseq sha3_512_64_ll (sha3_512_64_h' buf). qed.
 
 phoare sha_g buf: 
- [ Jkem768.M._sha3_512_64
+ [ Jkem768.M._sha3_512A_A64
  : arg.`2 = buf
  ==>
    let bytes = SHA3_512_64_64
